Linglib.lean
@@ -2485,9 +2485,7 @@ import Linglib.Syntax.DependencyGrammar.Dominance
 import Linglib.Syntax.DependencyGrammar.Length
 import Linglib.Syntax.DependencyGrammar.Projectivity
 import Linglib.Syntax.DependencyGrammar.Valency
-import Linglib.Syntax.HPSG.Basic
 import Linglib.Syntax.HPSG.Binding
-import Linglib.Syntax.HPSG.Categories
 import Linglib.Syntax.HPSG.Construction
 import Linglib.Syntax.HPSG.Description
 import Linglib.Syntax.HPSG.Interpretation
